Trying out P (Comp (P Value)) and getting stuck in continuity proof

coq/denot/continuity.v
@@ -1,49 +1,60 @@
-(* 
+(*
 
 This section proves that the denotation function is monotonic and continuous.
 
 Monotonicity
 
-   Definition monotone (F : P Value -> P Value) : Set := 
-         forall D1 D2, (D1 ⊆ D2) -> F D1 ⊆ F D2.
+   Definition monotone (F : P Value -> P Value) : Set := forall D1 D2, (D1 ⊆
+         D2) -> F D1 ⊆ F D2.
 
-   Lemma denot_monotone_one : forall ρ t x, 
-    uniq ρ -> x `notin` dom ρ ->
+   Lemma denot_monotone_one : forall ρ t x, uniq ρ -> x `notin` dom ρ ->
     monotone (fun D => denot (t ^ x) (x ~ D ++ ρ)).
 
 Continuity:
 
-   A semantic function is continuous if its finite result can be produced
-   by a finite and valid subset of its input.
+   A semantic function is continuous if any finite subset of any result of X
+   can be produced by a finite and valid subset of X.
 
-   Alex: this is algebraicity, equivalent to continuity for this kind of model.
-   To produce a finite output you only need a finite input.
+   [Alex notes: this is algebraicity, equivalent to continuity for this kind
+   of model.  To produce a finite output you only need a finite input.]
    
-   Definition continuous (F : P Value -> P Value) : Set :=
-     forall (X : P Value) (E : list Value), 
-           mem E ⊆ F X -> valid X ->
-           exists (D : list Value), 
-               (mem D ⊆ X) /\ ((mem E) ⊆ F (mem D)) /\ valid_mem D.
+   If our functions only concerned sets of values, then we might define
+   continuous as:
 
-   Lemma denot_continuous_one { t ρ x } :
-     valid_env ρ ->
-     x `notin` dom ρ ->
-     continuous (fun D => denot (t ^ x) (x ~ D ++ ρ)).
+        Definition continuous (F : P Value -> P Value) : Set := 
+          forall (X : P Value) (E : Comp (list B)), 
+             mem E ⊆ F X -> valid X -> 
+                exists (D : list Value), 
+                    (mem D ⊆ X) /\ ((mem E) ⊆ F (mem D)) /\ valid_mem D.
 
-The payoff for this section is a lemma for understanding how LAMBDA and APPLY interact.
-The general lemma looks like this:
+   However, our denotation function, used in the following lemma,
 
-Lemma Λ_APPLY_id { F X } :
-  continuous F -> monotone F -> valid X ->
-  (Λ F) ▩ X ≃ F X.
+       Lemma denot_continuous_one { t ρ x } : valid_env ρ 
+          -> x `notin` dom ρ
+          -> continuous (fun D => denot (t ^ x) (x ~ D ++ ρ)).
 
-With the above results, we can instantiate it to reason about the denotation function.
+   has type `P Value -> P (Comp (P Value))`.
 
-Lemma Λ_denot_APPLY_id : forall t ρ x X,
-    valid X ->
-    valid_env ρ ->
-    x `notin` dom ρ ->
-    ((Λ (fun D => denot (t ^ x) (x ~ D ++ ρ))) ▩ X) ≃ denot (t ^ x) (x ~ X ++ ρ).
+   Furthermore, in showing that this function is continuous, we also need to
+   reason about the continuity of the 'bind' operator.
+
+Why continuous and monotone?
+   
+   The payoff for this section is a lemma for understanding how LAMBDA and
+   APPLY interact.  The general lemma looks like this:
+
+        Lemma Λ_APPLY_id { F X } : 
+             continuous F -> monotone F -> valid X -> 
+             (Λ F) ▩ X ≃ F X.
+
+   With the above results, we can instantiate it to reason about the denotation
+   function.
+
+        Lemma Λ_denot_APPLY_id : forall t ρ x X, 
+            valid X -> 
+            valid_env ρ -> x `notin` dom ρ -> 
+               ((Λ (fun D => denot (t ^ x) (x ~ D ++ ρ))) ▩ X) 
+                 ≃ denot (t ^ x) (x ~ X ++ ρ).
 
  *)
 Require Import Coq.Logic.FunctionalExtensionality.
@@ -68,24 +79,12 @@ Open Scope tm.
 
 Import EnvNotations.
 
-(* Definitions related to continuity *)
+Lemma In_Sub {A}{x:A}{D}: x ∈ D <-> mem (x :: nil) ⊆ D.
+Proof. split. intros h y yIn. inversion yIn. subst; auto. inversion H. 
+       intros h. cbv in h. specialize (h x). tauto.
+Qed.
 
-Definition continuous {B} (F : P Value -> P B) : Set :=
-  forall X E, mem E ⊆ F X -> valid X 
-         -> exists D, (mem D ⊆ X) /\ ((mem E) ⊆ F (mem D)) /\ valid_mem D.
-
-Definition finite_env : Rho -> Type := Env.ForallT finite.
-
-Definition continuous_In {B} (D:Rho -> P B) (ρ:Rho) (v:B) : Prop :=
-  v ∈ D ρ -> exists ρ' , exists (pf : finite_env ρ'),  ρ' ⊆e ρ /\ (v ∈ D ρ').
-
-Definition continuous_Included {B} (D:Rho -> P B) (ρ:Rho) (X: P B) : Prop :=
-  finite X -> X ⊆ D ρ -> exists ρ' , exists (pf : finite_env ρ'),  ρ' ⊆e ρ /\ (X ⊆ D ρ').
-
-Definition continuous_env {B} (D:Rho -> P B) (ρ:Rho) : Prop :=
-  forall v, continuous_Included D ρ v.
-
-(* -------------------------------------- *)
+#[export] Hint Resolve In_Sub:core.
 
 
 Ltac gather_atoms ::=
@@ -96,18 +95,183 @@ Ltac gather_atoms ::=
   let E := gather_atoms_with (fun x : Rho => dom x) in
   constr:(A \u B \u C \u D \u E).
 
-(* -------------------------------------- *)
+
+Lemma denot_val_lit : forall k ρ,  denot_val (lit k) ρ = (NAT k).
+Proof. intros. reflexivity. Qed. 
+
+Lemma denot_val_add : forall ρ,  denot_val add ρ = ADD.
+Proof. intros. reflexivity. Qed. 
+
+Lemma denot_val_tnil : forall ρ,  denot_val tnil ρ = NIL.
+Proof.  intros. reflexivity. Qed. 
 
 
-(* -- monotonicity -- *)
-
-(*
-Lemma access_monotone {ρ ρ':Rho}{x} : ρ ⊆e ρ' -> ρ ⋅ x ⊆ ρ' ⋅ x.
+Lemma denot_val_abs : forall x t ρ,
+    x `notin` dom ρ \u fv_tm t ->
+    denot_val (abs t) ρ = 
+      (Λ2 (fun D => denot (t ^ x) (x ~ D ++ ρ))).
 Proof.
-  induction 1. simpl. reflexivity.
-  simpl. destruct (x == x0) eqn:E. auto.
-  auto. 
-Qed. *)
+  intros.
+  unfold denot_val,denot. simpl.
+  rewrite size_tm_open_tm_wrt_tm_var.
+  f_equal. f_equal.
+  extensionality D.
+  name_binder x0 Frx0.
+  simpl_env. 
+  rewrite -> (rename_open_denot x0 x); eauto.
+Qed.
+
+Lemma denot_val_tcons : forall t u ρ, 
+    denot_val (tcons t u) ρ = CONS (denot_val t ρ) (denot_val u ρ).
+Proof. 
+  intros.
+  unfold denot_val. simpl.
+  f_equal.
+  rewrite size_is_enough_val. lia. auto.
+  rewrite size_is_enough_val. lia. auto.
+Qed.
+
+
+#[export] Hint Rewrite denot_val_var denot_val_lit 
+  denot_val_add denot_val_tnil denot_val_tcons : denot.
+
+#[export] Instance Proper_sub_denot_val : Proper (eq ==> Env.Forall2 Included ==> Included) denot_val.
+Proof.
+  intros t1 t ->.
+  eapply tm_induction with (t := t);
+  [move=>i|move=>x|move=>t1 t2 IH1 IH2|move=> t' IH|move=>k| | | move=> t1 t2 IH1 IH2].
+  all: move => ρ1 ρ2 SUB.
+  all: autorewrite with denot.
+  all: try solve  [ simpl; reflexivity].
+  + eapply access_mono_sub; eauto.
+  + pick fresh x. 
+    repeat rewrite(denot_val_abs x). fsetdec. fsetdec.
+    eapply Λ_ext_sub.
+    intros X neX.
+    have SUBe: (x ~ X ++ ρ1) ⊆e (x ~ X ++ ρ2).
+    econstructor; eauto. reflexivity.
+    eapply Proper_sub_denot; eauto. 
+  + eapply CONS_mono_sub; eauto.
+Qed. 
+
+(* Definitions related to continuity 
+
+   For every finite approximation of an output, there is a finite approximation
+   of an input.
+
+   If the type is P Value, then the approx is list Value
+   If the type is P (Comp (P Value)), then the approx is list (Comp (list Value))
+
+*)
+
+Definition continuous {A} (F : P Value -> P A) : Set :=
+  forall X E, mem E ⊆ F X -> valid X 
+         -> exists D, (mem D ⊆ X) /\ ((mem E) ⊆ F (mem D)) /\ valid_mem D.
+
+Definition finite_env : Rho -> Type := Env.ForallT finite.
+
+Definition continuous_In {A} (D:Rho -> P A) (ρ:Rho) (v:A) : Prop :=
+  v ∈ D ρ -> exists ρ' , exists (pf : finite_env ρ'),  ρ' ⊆e ρ /\ (v ∈ D ρ').
+
+Definition continuous_env {A} (D:Rho -> P A) (ρ:Rho) : Prop :=
+  forall (v : A), continuous_In D ρ v.
+
+(* ----- Definitions for continuity --- functions that return computations *)
+
+(* Note: this is not the same as `inj C ⊆ D`, the sets in c_multi may 
+   be subsets of the sets in D. *)
+Definition Approx (C : list (Comp (list Value))) (D: P (Comp (P Value))) : Prop :=
+  forall c, List.In c C -> Comp_Approx_in c D.
+
+Lemma Comp_Approx_mem {A} : forall (c : Comp (list A)),  Comp_Approx c (fmap mem c).
+intros. destruct c. 
+all: econstructor; eauto.
+induction l.
+- simpl; auto.
+- simpl. econstructor. reflexivity. auto.
+Qed. 
+
+Lemma Comp_inj_Approx : forall C, Approx C (Comp_inj C).
+Proof.
+  intros. destruct C. cbv. intros. done.
+  unfold Approx. intros. destruct H. subst.
+  exists (fmap mem c0). split; eauto. unfold Comp_inj. cbn. left.  auto.
+  destruct c0. simpl. econstructor; eauto. 
+  econstructor; eauto.
+  induction l. simpl. auto.
+  econstructor; eauto. reflexivity.
+  exists (fmap mem c0).
+  split.
+  cbn. right.
+  eapply in_map. auto.
+  eapply Comp_Approx_mem; eauto.
+Qed.
+ 
+Definition continuous_M (F : P Value -> M (P Value)) : Set :=
+  forall X E, Approx E (F X) -> valid X 
+         -> exists D, (mem D ⊆ X) /\ (Approx E (F (mem D))) /\ valid_mem D.
+
+(* ----- Definitions for generalized continuty --- any input, any output *)
+
+(* A type can be finitely approximated by another type if there is 
+   an injection and a relation. 
+   There are probably some properties we need from these definitions,
+   but I'm note sure what they are yet.
+*)
+Class FinApprox (A : Type) := 
+  { Finite : Type; 
+    inj    : Finite -> A; 
+    approx : Finite -> A -> Prop 
+  }.
+
+Infix "⊑" := approx (at level 65).
+
+(* Approximate sets of values by lists of values *)
+#[global] Instance FAV : FinApprox (P Value) := 
+  { Finite := list Value; 
+    inj    := mem; 
+    approx := fun l X => mem l ⊆ X }.
+
+(* Approximate valid sets of values by valid lists of values *)
+#[global] Instance FAVNE : FinApprox { x : P Value & valid x } := 
+  { Finite := { x : list Value & valid_mem x }; 
+    inj := fun x => match x with
+                   | existT _ y z => existT _ (mem y) (valid_mem_valid z)
+                 end;
+    approx := fun l X => mem (projT1 l) ⊆ (projT1 X) }.
+
+(* Approximate computations *)
+#[global] Instance FAC : FinApprox (P (Comp (P Value))) := 
+  { Finite := list (Comp (list Value));
+    inj    := Comp_inj;
+    approx := Approx
+  }.
+
+(* Approximate environments by finite environments *)
+#[global] Instance FAR : FinApprox Rho := 
+  { Finite    := { ρ & finite_env ρ };
+    inj       := @projT1 Rho finite_env;
+    approx    := fun x y => Env.Forall2 Included (projT1 x) y
+  }.
+
+(* A function F is continuous for an argument X, if for all finite approximations 
+   of the result, there is a finite approximation of X that returns the same
+   result. *)
+Definition continuous_For {A B :Type}`{FinApprox A}`{FinApprox B} (F : A -> B)
+  (X : A) : Prop :=
+  forall (E : Finite), E ⊑ F X -> exists (D : Finite), (D ⊑ X) /\ (E ⊑ F (inj D)).
+
+(* A function F is continuous if it is continuous for every argument. *)
+Definition continuous' {A B :Type}`{FinApprox A}`{FinApprox B} (F : A -> B) : Prop :=
+  forall X, continuous_For F X.
+
+(* Functions that are continuous for a specific environment. *)
+Definition continuous_env' {A}`{FinApprox A}(F : Rho -> A) : Rho -> Prop :=
+  continuous_For F.
+
+
+
+(* -- monotonicity WRT environments -- *)
 
 (*  forall ρ ρ', ρ ⊆e ρ' -> denot t ρ ⊆ denot t ρ'. *)
 Lemma denot_monotone {t}: 
@@ -118,7 +282,15 @@ Proof.
   eapply Proper_sub_denot; auto.
 Qed.
 
+Lemma denot_val_monotone {t}: 
+  monotone_env (denot_val t).
+Proof.
+  unfold monotone_env.
+  intros. 
+  eapply Proper_sub_denot_val; auto.
+Qed.
 
+(* -- monotonicity WRT argument -- *)
 (* denot-monotone-one *)
 Lemma denot_monotone_one : forall ρ t x, 
     uniq ρ -> x `notin` dom ρ ->
@@ -306,7 +478,6 @@ Proof.
     ++ econstructor; eauto. 
        eapply IHNE; eauto. fsetdec.
        simpl_env. auto.
-       intros y h. inversion h. subst. unfold In. auto.
 Qed.
 
 #[export] Hint Resolve single_sub : core. 
@@ -342,9 +513,11 @@ Qed.
 
 #[export] Hint Resolve v_single_xvx : core. 
 
+
+
 (* continuous-∈⇒⊆ *)
-(*
-Lemma continuous_In_sub {A} (E : Rho -> (P A)) ρ (NE : valid_env ρ) :
+
+Lemma continuous_In_sub (E : Rho -> (P Value)) ρ (NE : valid_env ρ) :
    monotone_env E
    -> forall V, mem V ⊆ E ρ
    -> (forall v, v ∈ mem V -> continuous_In E ρ v)
@@ -376,12 +549,285 @@ Proof.
     eapply me. eapply join_sub_right; eauto. auto. 
     eapply me. eapply join_sub_left; eauto. auto.
 Qed.
-*)
+
+
+
+Lemma continuous_In_sub' (E : Rho -> M (P Value)) ρ (NE : valid_env ρ) :
+   monotone_env E
+   -> continuous_For E ρ
+   -> forall V, V ⊑ E ρ
+   -> exists ρ', exists (pf : finite_env ρ') ,  ρ' ⊆e ρ /\ (V ⊑ E ρ').
+Proof.
+  intros me vcont V VE.
+  unfold continuous_For in vcont.
+  specialize (vcont V VE).
+  move: vcont => [ [ρ' fρ'] [h1 h2]].
+  cbn in h1.
+  cbn in h2.
+  eexists ρ'. eexists. auto.
+  split; eauto.
+Qed.
+
+(*  induction V.
+  - exists (initial_finite_env ρ NE).
+    repeat split.
+    eapply (initial_fin ρ NE).
+    eapply initial_fin_sub; eauto. 
+    done.
+  - 
+    
+    destruct IHV as [ ρ1 [ fρ1 [ ρ1ρ VEρ1 ]]].
+    intros d D inV inE.
+    eapply VE; eauto. simpl. right; auto.
+
+   
+    destruct (vcont a) as [ρ2 [fρ2 [ρ2ρ VEρ2]]].
+    econstructor; eauto.
+    eapply VE. econstructor; eauto.
+    exists (ρ1 ⊔e ρ2).
+    have S1: same_scope ρ1 ρ. eapply Forall2_same_scope; eauto.
+    have S2: same_scope ρ2 ρ. eapply Forall2_same_scope; eauto. 
+    have SS: same_scope ρ1 ρ2. 
+    { transitivity ρ; auto. symmetry; auto. }
+    eexists. eapply join_finite_env; eauto.
+    repeat split.
+    + eapply join_lub; eauto.
+    + intros d dm.
+    inversion dm; subst.
+    eapply me. eapply join_sub_right; eauto. auto. 
+    eapply me. eapply join_sub_left; eauto. auto.
+Qed. *)
+
+
+
 (* --------------------------------------- *)
 
 (* Operations are continuous *)
 
-Search Singleton.
+Lemma mem_injective {A} {l1 l2 : list A} : mem l1 = mem l2 -> l1 = l2.
+Proof. 
+  move: l2. induction l1; intros l2 h; destruct l2; try done.
+  unfold mem in h.
+Admitted.
+
+Lemma map_mem_injective {A}{l l0 : list (list A)} :
+  List.map mem l = List.map mem l0 -> l = l0.
+Proof.
+  move: l0.
+  induction l; intro l0; destruct l0; intro h; try done.
+  simpl in h. inversion h.  
+  eapply mem_injective in H0.
+  eapply IHl in H1; eauto.
+  f_equal; auto.
+Qed.
+
+Lemma fmap_Comp_mem_injective {w0 w : Comp (list Value)} 
+  : fmap_Comp mem w0 = fmap_Comp mem w -> w0 = w.
+Proof.
+  intro h.
+  destruct w0; destruct w; try done.
+  inversion h.
+  apply map_mem_injective in H0.
+  f_equal; auto.
+Qed.
+
+Lemma singleton_mem_singleton {A}{w:A}{l} :
+ ⌈ w ⌉ = mem l -> l = (w :: nil).
+Proof.
+  destruct l; unfold mem.
+  intro h.
+  have h1: ⌈ w ⌉ w = (fun x : A => In x nil) w.
+  rewrite h. auto.
+  simpl in h1. 
+  have h2:  ⌈ w ⌉ w. eapply in_singleton. rewrite h1 in h2. done.
+  intro h.
+  have h1: ⌈ w ⌉ w = (fun x : A => In x (a :: l)) w.
+  rewrite h. done.
+  have h2:  ⌈ w ⌉ w. eapply in_singleton. rewrite h1 in h2.
+  inversion h2. subst. 
+Admitted.
+
+Lemma APPLY_continuous {D E ρ}{w : Comp (list Value)} :
+  (valid_env ρ)
+  -> fmap mem w ∈ (D ρ ▩ E ρ)
+  -> continuous_env D ρ 
+  -> continuous_env E ρ
+  -> monotone_env D 
+  -> monotone_env E
+  -> exists ρ' , 
+    exists (pf : finite_env ρ') , ρ' ⊆e ρ /\ (fmap mem w ∈ (D ρ' ▩ E ρ')).
+Proof.  
+  intros NE APP. inversion APP; subst. 
+  all: intros IHD IHE mD mE.
+  + apply fmap_Comp_mem_injective in H; subst.
+    destruct (IHD ( V ↦ w ) ltac:(auto)) (* finite_Singleton (In_Included H)) *) as 
+      [ ρ1 [ fρ1 [ ρ1ρ VwDp1 ]]].
+    destruct 
+      (continuous_In_sub E ρ NE mE V)
+      as [ ρ2 [ fρ2 [ ρ2ρ VEp2 ]]]; eauto.
+    have S1: same_scope ρ1 ρ. eapply Forall2_same_scope; eauto.
+    have S2: same_scope ρ2 ρ. eapply Forall2_same_scope; eauto.
+    have SS: same_scope ρ1 ρ2. { transitivity ρ; auto. symmetry; auto. }
+    exists (ρ1 ⊔e ρ2).
+    repeat split.
+  - eapply join_finite_env; eauto.
+  - eapply join_lub; eauto.
+  - have VwDp3 : ⌈ V ↦ w ⌉ ⊆ D (ρ1 ⊔e ρ2).
+    { transitivity (D ρ1); auto. eapply mD. 
+      eapply join_sub_left. auto. }
+    have VEρ3 : mem V ⊆ E (ρ1 ⊔e ρ2).
+    { transitivity (E ρ2); auto. eapply mE.
+      eapply join_sub_right.  auto. }
+    eapply BETA with (V:=V); auto.
+ + unfold pure_Comp in H; destruct w; try done.
+   destruct l; try destruct l0; try done. 
+   simpl in H. inversion H. apply singleton_mem_singleton in H3.
+   subst. clear H.
+   destruct (IHD (v_list VS) ) as [ρ1 [F1 [h1 h2]]]; auto.
+   destruct (IHE (v_nat k) ) as [ρ2 [F2 [h3 h4]]]; auto.
+    have S1: same_scope ρ1 ρ. eapply Forall2_same_scope; eauto.
+    have S2: same_scope ρ2 ρ. eapply Forall2_same_scope; eauto.
+    have SS: same_scope ρ1 ρ2. { transitivity ρ; auto. symmetry; auto. }
+   exists (ρ1 ⊔e ρ2).
+    repeat split.
+  - eapply join_finite_env; eauto.    
+  - eapply join_lub; eauto.
+  - cbn. 
+    replace (mem (w0 :: nil)) with ⌈ w0 ⌉. 
+    eapply PROJ with (VS := VS) (k:=k); eauto.
+    eapply mD. eapply join_sub_left; auto. auto.
+    eapply mE. eapply join_sub_right; auto. auto.
+    eapply Extensionality_Ensembles.
+    split; eauto. 
+ + destruct w; try done. 
+   destruct (IHD x) as [ρ1 [F1 [h1 h2]]]; auto.
+    eexists.
+    eexists.
+    eauto.
+    split; eauto.
+    eapply APPWRONG with (x:=x); auto.
+ + destruct w; try done. 
+   destruct (IHE x) as [ρ2 [F1 [h1 h2]]]; auto.
+    destruct (IHD (v_list VS)) as [ρ1 [F2 [h01 h02]]]; auto.
+    have S1: same_scope ρ1 ρ. eapply Forall2_same_scope; eauto.
+    have S2: same_scope ρ2 ρ. eapply Forall2_same_scope; eauto.
+    have SS: same_scope ρ1 ρ2. { transitivity ρ; auto. symmetry; auto. }
+    exists (ρ1 ⊔e ρ2).
+    repeat split.
+    - eapply join_finite_env; eauto.    
+    - eapply join_lub; eauto.
+    - eapply PROJWRONG with (VS := VS); eauto.
+    eapply mD. eapply join_sub_left; auto. auto.
+    eapply mE. eapply join_sub_right; auto. auto.
+Qed.
+
+
+
+Lemma env_tail {ρ' x v ρ} :  
+  ρ' ⊆e (x ~ v ++ ρ) -> finite_env ρ' -> 
+  nonempty_env ρ ->
+  exists w, exists ρ'', ρ' = (x ~ w ++ ρ'') /\
+                (w ⊆ v) /\
+                exists (pf : finite_env ρ''), 
+                ρ'' ⊆e ρ.                
+Proof.
+  intros h k ne.
+  inversion h. subst.
+  exists a1.  exists E1.
+  repeat split; auto. inversion k.  auto.
+Qed.
+
+(* Algebraicity.  
+   Only need finite information from the environment.
+*)
+
+Lemma In_Approx {c : Comp (list Value)}{E : M (P Value)} :
+ fmap mem c ∈ E -> Approx (c :: nil) E.
+Proof.
+  unfold Approx.
+  intros. simpl in H0. destruct H0; try done; subst.
+  exists (fmap mem c0). 
+  split; eauto.
+  eapply Comp_Approx_mem.
+Qed.
+
+Lemma Lambda_continuous {E ρ x} {NE : valid_env ρ}{v} :
+  v ∈ Λ2 (fun D => E (x ~ D ++ ρ)) 
+  -> x `notin` dom ρ
+  -> (forall V, valid_mem V -> continuous_env' E (x ~ mem V ++ ρ))
+  -> monotone_env E
+  -> exists ρ', exists (pf:finite_env ρ'),
+            ρ' ⊆e ρ /\ (v ∈ (Λ2 (fun D => E (x ~ D ++ ρ')))).
+Proof.
+Admitted.
+(*
+  induction v.
+  all: try solve [intros; cbv in H; done].
+  - (* v is l ↦ c *)
+    intros [ wEVρ NW ] Fr IH mE.
+
+    have VV: valid_mem l. unfold valid_mem. eauto.
+    have NEx: valid_env (x ~ mem l ++ ρ). econstructor; eauto.
+
+    specialize (IH l ltac:(eauto)).
+
+    unfold continuous_env', continuous_For, Finite, FAC, FAR in IH.
+
+    move: (IH (c :: nil)) => h.
+    destruct h as [ [ρ' fρ'] [ ρ'Vρ wEρ' ]]. 
+    { eapply In_Approx. auto. }
+
+    simpl in wEρ'. unfold Approx in wEρ'.
+    specialize (wEρ' c). 
+    destruct wEρ' as [d [dIn apx]]. simpl; left; auto.
+
+    inversion ρ'Vρ. simpl in H2. subst. clear ρ'Vρ. 
+    inversion fρ'. subst.  clear fρ'.
+
+    exists E1. exists X.
+    split. eauto.
+    cbn. split; auto.
+
+    have SE: (x ~ a1 ++ E1) ⊆e (x ~ mem l ++ E1).
+    econstructor; eauto. eapply Reflexive_sub_env. eapply Forall2_uniq1; eauto.
+    eapply mE. eapply SE. clear SE.
+
+    inversion apx; subst. simpl; eauto.
+    
+    
+
+    unfold continuous_env', continuous_For in IH.
+    unfold Finite, FAC, FAR in IH.
+
+    have KK: mem (fmap_Comp mem c :: nil) ⊑ E (x ~ mem l ++ ρ).
+    { intros xx xxIn. cbn in xxIn. destruct xxIn; try done. subst. auto. }
+
+    move: (continuous_In_sub E (x ~ mem l ++ ρ) NEx mE (fmap_Comp mem c :: nil) KK) => h.
+
+    move: (IH l ltac:(eauto)) => IH'. 
+    
+
+    edestruct IH' as [ρ' fp'].
+[ ρ' [ fρ' [ ρ'Vρ wEρ' ]]]. 
+hh.
+    destruct hh as [ ρ' [ fρ' [ ρ'Vρ wEρ' ]]].
+    intros v vIn. eapply IH. auto.
+(*    destruct (IH l ltac:(eauto) ⌈ c ⌉ finite_Singleton (In_Included wEVρ)) as
+      [ ρ' [ fρ' [ ρ'Vρ wEρ' ]]].  *)
+    inversion ρ'Vρ. subst. clear ρ'Vρ.
+    inversion fρ'. subst. clear fρ'.
+    exists E1. exists X.
+    repeat split; eauto.
+    specialize (wEρ' (fmap mem c)). 
+    eapply mE. 2: eapply wEρ'.
+    have SS: E1 ⊆e E1. eapply Reflexive_sub_env.  eapply Forall2_uniq1; eauto. 
+    auto.
+    eauto.
+  - exists (initial_finite_env ρ NE).
+    repeat split; eauto.
+Qed.
+
+*)
 
 Lemma In_Included : forall {A}{x:A}{D},  x ∈ D -> ⌈ x ⌉ ⊆ D.
 Proof. 
@@ -417,6 +863,8 @@ Proof.
   destruct l. try done.
   move: C => [Dv El].
   intros IHD IHE mD mE.
+Admitted.
+(*
   destruct (IHD ⌈ v ⌉ finite_Singleton (In_Included Dv)) as 
       [ ρ1 [ fρ1 [ ρ1ρ VwDp1 ]]].
   destruct (IHE ⌈ v_list l ⌉ finite_Singleton (In_Included El)) as 
@@ -432,164 +880,66 @@ Proof.
     eapply join_sub_left; eauto. auto.
   - eapply mE. instantiate (1:= ρ2).
     eapply join_sub_right; eauto. auto.
-Qed.
+Qed. *)
 
 
+(* ---- RET : P Value -> M (P Value) ----- *)
 
-(*  BIND2 S K := exists U : P A, (RET2 U ⊆ S) /\ K U t *)
-
-Lemma BIND2_continuous {A B}{D : Rho -> M A}{K : P A -> M B}{ρ}{v} :
+Lemma RET_continuous {D: Rho -> (P Value)}{ρ}{c} : 
   valid_env ρ ->
-  v ∈ BIND2 (D ρ) K -> 
-  continuous_env D ρ ->
+  continuous_env' D ρ ->
+  monotone_env D ->
+  c ∈ RET (D ρ) ->
+  forall (x : Comp (list Value)), Comp_Approx x c ->
+    exists (ρ' : Rho), 
+    exists _ :(finite_env ρ'), (ρ' ⊆e ρ) /\ (fmap mem x ∈ RET (D ρ')).
+Proof.
+  intros VE CE ME cIn x SU.
+  destruct c; try destruct l as [|V l] ; try destruct l; cbn in cIn; try done.
+  inversion SU. subst. inversion H1. subst. inversion H4. subst.
+  clear H1 H4 SU.
+  unfold continuous_env', continuous_For in *.
+Admitted.
+
+
+(*
+Lemma BIND_continuous {A B}{D : Rho -> P (Comp (P A))}{K : Rho -> P A -> P (Comp (P B))}{ρ}{v} :
+  valid_env ρ ->
+  v ∈ BIND (D ρ) (K ρ) -> 
+  continuous_env' D ρ ->
   monotone_env D  ->
-  forall E, K = (fun v => E v ρ) ->
-  (forall v, continuous_env (E v) ρ) ->
-  (forall v, monotone_env (E v)) ->
+  (forall v, continuous_env (fun r => K r v) ρ) ->
+  (forall v, monotone_env (fun r => K r v)) ->
   exists ρ', exists (pf:finite_env ρ'),
-            ρ' ⊆e ρ /\ (v ∈ BIND2 (D ρ') (fun v => E v ρ')). 
+            ρ' ⊆e ρ /\ (v ∈ BIND (D ρ') (K ρ')). 
 Proof.
-  intros VE H IHD mD E -> IHE mE. 
-  move: H => [U [h1 [h2 h3]]].
-  specialize (IHE U).
-  specialize (mE U).
-  have NE : finite (RET2 U). { inversion h1. destruct H. unfold RET2. econstructor; eauto. rewrite H. 
-                               instantiate (1 := fmap pure_Comp x). split. admit. admit. }
-  edestruct (IHD _  NE h2) as 
+  intros VE H IHD mD IHE mE. 
+  move: H => [U [h1 [h2 [-> h3]]]].
+  unfold continuous_env, continuous_In in IHD.
+  edestruct (IHD U ltac:(eauto)) as 
       [ ρ1 [ fρ1 [ ρ1ρ VwDp1 ]]].
-  edestruct (IHE ⌈ v ⌉ finite_Singleton (In_Included h3)) as 
-      [ ρ2 [ fρ2 [ ρ2ρ VwDp2 ]]].
-  have S1: same_scope ρ1 ρ. eapply Forall2_same_scope; eauto.
-  have S2: same_scope ρ2 ρ. eapply Forall2_same_scope; eauto.
-  have SS: same_scope ρ1 ρ2. { transitivity ρ; auto. symmetry; auto. }
-  exists (ρ1 ⊔e ρ2).
-  repeat split.
-  + eapply join_finite_env; eauto.
-  + eapply join_lub; eauto.
-  + unfold Ensembles.In.
-    unfold BIND2.
-    exists U. repeat split. auto. transitivity (D ρ1). auto.
-    eapply mD.
-    eapply join_sub_left; eauto.
-    eapply Included_In.
-    transitivity (E U ρ2); auto.
-    apply mE. eapply join_sub_right; eauto. 
-Admitted.
+  destruct U.
+  + exists ρ1. repeat split; eauto.
+    cbn.
+    unfold BIND. 
+    exists c_wrong. exists (fun x => c_wrong).
+    repeat split; eauto.
+    intros x h. inversion h.
+  + (* need a lemma about all of the VS in the list l. *)
+     admit.    
+  + exists ρ1. repeat split; eauto.
+    cbn.
+    unfold BIND. 
+    exists c_bottom. exists (fun x => c_bottom).
+    repeat split; eauto.
+    intros x h. inversion h.
+Admitted. 
 
-Lemma APPLY_continuous {D E ρ}{w} :
-  (valid_env ρ)
-  -> w ∈ ((D ρ) ▩ (E ρ))
-  -> continuous_env D ρ 
-  -> continuous_env E ρ
-  -> monotone_env D 
-  -> monotone_env E
-  -> exists ρ3 , 
-    exists (pf : finite_env ρ3) , ρ3 ⊆e  ρ 
-                             /\ (w ∈ ((D ρ3) ▩ (E ρ3))).
-Proof.  
-  intros NE APP. inversion APP; subst. 
-  all: intros IHD IHE mD mE.
-  + destruct (IHD ⌈ V ↦ w ⌉ finite_Singleton (In_Included H)) as 
-      [ ρ1 [ fρ1 [ ρ1ρ VwDp1 ]]].
-    have NEV: finite (mem V). admit. (* {  unfold valid_mem in H1. destruct V; try done. econstructor; eauto. } *)
-    destruct (IHE (mem V) ltac:(eauto) H0) as 
-      [ ρ2 [ fρ2 [ ρ2ρ VEp2 ]]]; eauto.
-    have S1: same_scope ρ1 ρ. eapply Forall2_same_scope; eauto.
-    have S2: same_scope ρ2 ρ. eapply Forall2_same_scope; eauto.
-    have SS: same_scope ρ1 ρ2. { transitivity ρ; auto. symmetry; auto. }
-    exists (ρ1 ⊔e ρ2).
-    repeat split.
-  - eapply join_finite_env; eauto.
-  - eapply join_lub; eauto.
-  - have VwDp3 : ⌈ V ↦ w ⌉ ⊆ D (ρ1 ⊔e ρ2).
-    { transitivity (D ρ1); auto. eapply mD. 
-      eapply join_sub_left. auto. }
-    have VEρ3 : mem V ⊆ E (ρ1 ⊔e ρ2).
-    { transitivity (E ρ2); auto. eapply mE.
-      eapply join_sub_right.  auto. }
-    eapply BETA with (V:=V); auto.
- + destruct (IHD ⌈ v_list VS ⌉ ) as [ρ1 [F1 [h1 h2]]]; auto using In_Included, finite_Singleton.
-   destruct (IHE ⌈ v_nat k ⌉ ) as [ρ2 [F2 [h3 h4]]]; auto using In_Included, finite_Singleton.
-    have S1: same_scope ρ1 ρ. eapply Forall2_same_scope; eauto.
-    have S2: same_scope ρ2 ρ. eapply Forall2_same_scope; eauto.
-    have SS: same_scope ρ1 ρ2. { transitivity ρ; auto. symmetry; auto. }
-   exists (ρ1 ⊔e ρ2).
-    repeat split.
-  - eapply join_finite_env; eauto.    
-  - eapply join_lub; eauto.
-  - eapply PROJ with (VS := VS) (k:=k); eauto.
-    eapply mD. eapply join_sub_left; auto. auto.
-    eapply mE. eapply join_sub_right; auto. auto.
- +  destruct (IHD ⌈ x ⌉) as [ρ1 [F1 [h1 h2]]]; auto using In_Included, finite_Singleton.
-    eexists.
-    eexists.
-    eauto.
-    split; eauto.
-    eapply APPWRONG with (x:=x); auto.
- +  destruct (IHE ⌈ x ⌉) as [ρ2 [F1 [h1 h2]]]; auto using In_Included, finite_Singleton.
-    destruct (IHD ⌈ v_list VS ⌉) as [ρ1 [F2 [h01 h02]]]; auto using In_Included, finite_Singleton.
-    have S1: same_scope ρ1 ρ. eapply Forall2_same_scope; eauto.
-    have S2: same_scope ρ2 ρ. eapply Forall2_same_scope; eauto.
-    have SS: same_scope ρ1 ρ2. { transitivity ρ; auto. symmetry; auto. }
-    exists (ρ1 ⊔e ρ2).
-    repeat split.
-    - eapply join_finite_env; eauto.    
-    - eapply join_lub; eauto.
-    - eapply PROJWRONG with (VS := VS); eauto.
-    eapply mD. eapply join_sub_left; auto. auto.
-    eapply mE. eapply join_sub_right; auto. auto.
-Admitted.
-
-
-
-Lemma env_tail {ρ' x v ρ} :  
-  ρ' ⊆e (x ~ v ++ ρ) -> finite_env ρ' -> 
-  nonempty_env ρ ->
-  exists w, exists ρ'', ρ' = (x ~ w ++ ρ'') /\
-                (w ⊆ v) /\
-                exists (pf : finite_env ρ''), 
-                ρ'' ⊆e ρ.                
-Proof.
-  intros h k ne.
-  inversion h. subst.
-  exists a1.  exists E1.
-  repeat split; auto. inversion k.  auto.
-Qed.
-
-(* Algebraicity.  
-   Only need finite information from the environment.
 *)
-
-Lemma Lambda_continuous {E ρ} {NE : valid_env ρ}{ v x} :
-  v ∈ Λ (fun D => E (x ~ D ++ ρ)) 
-  -> (forall V, valid_mem V -> continuous_env E (x ~ mem V ++ ρ))
-  -> monotone_env E
-  -> exists ρ', exists (pf:finite_env ρ'),
-            ρ' ⊆e ρ /\  (v ∈ (Λ (fun D => E (x ~ D ++ ρ')))).
-Proof.
-  induction v.
-  all: try solve [intros; cbv in H; done].
-  - (* v is l ↦ v *)
-    intros [ wEVρ NW ] IH mE.
-    have VV: valid_mem l. unfold valid_mem. eauto.
-    destruct (IH l ltac:(eauto) ⌈ c ⌉ finite_Singleton (In_Included wEVρ)) as
-      [ ρ' [ fρ' [ ρ'Vρ wEρ' ]]]. 
-    inversion ρ'Vρ. subst. clear ρ'Vρ.
-    inversion fρ'. subst. clear fρ'.
-    exists E1. exists X.
-    repeat split; eauto.
-    eapply Included_In.
-    transitivity (E (x ~ a1 ++ E1)); auto.
-    eapply mE. 
-    have SS: E1 ⊆e E1. eapply Reflexive_sub_env.  eapply Forall2_uniq1; eauto. 
-    auto.
-  - exists (initial_finite_env ρ NE).
-    repeat split; eauto.
-Qed.
-
 
 (* ---------------- Denotation is continuous ----------------- *)
 
+(*
 Lemma Included_RET2 {A}{v:M A}{Y}: (v ⊆ RET2 Y) ->  exists X, (v ≃ RET2 X) /\ (X ⊆ Y).
 Proof.
   intros.
@@ -604,28 +954,66 @@ Proof.
   - intros y Iny.
     destruct Iny. auto.
 Qed.
-  
+  *)
 
 
-(* ⟦⟧-continuous *)
-Lemma denot_continuous {t} : forall ρ,
+(*
+Lemma denot_val_continuous {t} : forall ρ,
     valid_env ρ
-  -> continuous_env (denot t) ρ.
+  -> continuous_env (denot_val t) ρ.
 Proof.
   eapply tm_induction with (t := t);
   [move=>i|move=>x|move=>t1 t2 IH1 IH2|move=> t' IH|move=>k| | | move=> t1 t2 IH1 IH2].
   all: intros ρ NE.
-  all: intros m NEm mSub.
-  all: autorewrite with denot in mSub.
-  all: try solve [ exists (initial_finite_env ρ NE);
-    eexists; eauto] .
-  + exfalso. destruct NEm. admit. (* eapply mSub.  eauto.  *)
-  + move: (Included_RET2 mSub) => [X [E S]].
-    destruct (FSetDecideAuxiliary.dec_In x (dom ρ)).
-    - exists (single_env x X ρ NE).
-      split.
-      have FX: finite X. admit.
+  all: intros v vIn.
+  all: autorewrite with denot in vIn.
+  all: try solve [ exists (initial_finite_env ρ NE); eexists; eauto] .
+  - destruct (FSetDecideAuxiliary.dec_In x (dom ρ)).
+    + exists (single_env x ⌈ v ⌉ ρ NE).
+      repeat split.
       eapply single_fin; eauto.
+      eapply single_sub; eauto.
+      rewrite denot_val_var.
+      eapply v_single_xvx; eauto.
+    + rewrite access_fresh in vIn; auto.
+      inversion vIn.
+  - pick fresh x.
+    rewrite (denot_val_abs x) in vIn. fsetdec.
+    admit. (* Wrong IH. *)
+  - rewrite denot_val_tcons in vIn. 
+    eapply CONS_continuous in vIn; eauto.
+    move: vIn => [ρ' [F' [S' vIn']]].
+    exists ρ'. repeat split; auto.
+    rewrite denot_val_tcons. auto.
+*)
+
+(* ⟦⟧-continuous *)
+Lemma denot_continuous {t} : forall ρ,
+    valid_env ρ
+  -> continuous_env' (denot t) ρ.
+Proof.
+  eapply tm_induction with (t := t);
+  [move=>i|move=>x|move=>t1 t2 IH1 IH2|move=> t' IH|move=>k| | | move=> t1 t2 IH1 IH2].
+  all: intros ρ NE.
+  all: intros c cIn.
+  all: autorewrite with denot in cIn.
+  destruct c; cbn in cIn; unfold Approx in cIn.
+Admitted.
+(*
+   specialize (cIn c ltac:(econstructor; eauto)).
+   destruct cIn as [x [h0 h1]]; done.
+
+c(*   all: try solve [ exists (initial_finite_env ρ NE);
+    eexists; eauto] . *)
+  + cbn. exfalso. edestruct cIn.
+  + destruct c; try done.  destruct l as [|V l]; try done. destruct l; try done. 
+    cbn in cIn.
+    destruct (FSetDecideAuxiliary.dec_In x (dom ρ)).
+    - 
+      exists (single_env x v ρ NE).
+      split.
+      eapply single_fin; eauto.
+      Search finite valid_env.
       split.
       ++ eapply single_sub; auto.
       ++ rewrite denot_var. 
@@ -677,9 +1065,10 @@ Proof.
     exists ρ'. exists F.
     rewrite denot_tcons. auto.
 Qed.
-
+*)
 
 (* ⟦⟧-continuous-⊆ *) 
+(*
 Lemma denot_continuous_sub {ρ t} : 
   valid_env ρ
   -> forall V, mem V ⊆ denot t ρ
@@ -692,15 +1081,49 @@ Proof.
   intros v InV.
   eapply denot_continuous; auto.
 Qed.
+*)
+
+Lemma denot_continuous_sub {ρ t} : 
+  valid_env ρ
+  -> forall E, Approx E (denot t ρ)
+  -> exists ρ', exists (pf : finite_env ρ'),
+        ρ' ⊆e ρ  /\  (Approx E (denot t ρ')).
+Admitted.
+
+Definition implies (A B : Prop) : Prop := A -> B.
+
+#[global] Instance Proper_Approx : Proper (Logic.eq ==> Ensembles.Included ==> implies) Approx.
+intros x1 y1 -> x2 y2 S. 
+unfold Approx, implies in *.
+- intros h c cIn. specialize (h c cIn). 
+unfold Comp_Approx_in in *.
+move: h => [d [dIn s]].
+exists d. split. eauto. auto.
+Qed.
+
+Lemma Approx_sub : forall c X1 X2, X1 ⊆ X2 -> Approx c X1 -> Approx c X2.
+intros c X1 X2 S. 
+unfold Approx. 
+intros h d dIn. specialize (h d dIn). 
+unfold Comp_Approx_in in *.
+move: h => [e [eIn s]].
+exists e. split. eauto. auto.
+Qed.
+
+(* This doesn't work, because we need a finite description of the result *)
+Definition continuous_M' (F : P Value -> M (P Value)) : Set :=
+  forall X E, mem E ⊆ (F X) -> valid X 
+         -> exists D, (mem D ⊆ X) /\ (mem E ⊆ (F (mem D))) /\ valid_mem D.
+
 
 (* ⟦⟧-continuous-one *)
 Lemma denot_continuous_one { t ρ x } :
   valid_env ρ 
   -> x `notin` dom ρ 
-  -> continuous (fun D => denot (t ^ x) (x ~ D ++ ρ)).
+  -> continuous_M (fun D => denot (t ^ x) (x ~ D ++ ρ)).
 Proof.
   intros NE_ρ Fr.
-  unfold continuous.
+  unfold continuous_M.
   intros X E E_sub_denot NE_X.
   edestruct (@denot_continuous_sub (x ~ X ++ ρ)) as 
     [ρ' [pf [h1 h2]]]. 3: eauto.
@@ -714,7 +1137,8 @@ Proof.
     have SUB: Env.Forall2 Included (x ~ a1 ++ E1) (x ~ mem D ++ ρ).
     econstructor; eauto. 
     rewrite <- S. reflexivity.
-    rewrite <- SUB.
+    eapply Approx_sub. 2: eapply h2.
+    eapply denot_monotone.
     auto.
     eapply valid_sub_valid_mem; eauto. rewrite <- S. auto.
 Qed.
@@ -723,25 +1147,33 @@ Qed.
 
 (* Λ-▪-id *)
 Lemma Λ_APPLY_id { F X } :
-  continuous F -> monotone F -> valid X
-  -> (Λ F) ▩ X ≃ F X.
+  continuous_M F -> monotone F -> valid X
+  -> (Λ2 F) ▩ X ≃ F X.
 Proof. 
   intros Fcont Fmono NEX.
   split.
-  + intros w APP. inversion APP; subst. 
-    - inversion H.
-    - exfalso; eapply valid_not_wrong; eauto. 
-    - inversion H.
-      eapply (Fmono (mem V) X); eauto. 
-    - inversion H.
+  + intros w APP. inversion APP; subst.
+    - cbn in H. destruct H as [h1 h2].
+      specialize (Fmono (mem V) X ltac:(auto)).
+      eauto.
+    - cbn in H. try done.
     - destruct x; try done.
     - destruct x; try done.
   + intros w wInFX.
+
+    unfold continuous_M in Fcont.
+
+    destruct w. 
+    - admit.
+    - 
+
     have M: mem (cons w nil) ⊆ F X. 
     { intros d y. inversion y; subst. auto. done. }
+
     move: (Fcont X (cons w nil) M NEX) => 
     [ D [ DltX [ wInFD NED ]]].
-    move: NEX => [ [x h0] h1].
+
+
     eapply BETA with (V:=D); eauto.
     repeat split; eauto.
     eapply Forall_sub_mem; eauto.
