coq/denot/definitions.v
@@ -9,7 +9,6 @@
       valid : P Value -> Prop     (is the set nonempty & only contain successful values?)
 
    Semantic operators:
-
     WRONG : P Value   
 
     NAT   : nat -> P Value
@@ -52,19 +51,25 @@ Local Open Scope set_scope.
 
 (* ----------------------------------------------------------- *)
 
-(* Computations that can fail or produce multiple results. *)
+(* Computations that can fail, produce multiple results, or diverge. *)
 
 Inductive Comp (v : Type) : Type := 
   (* dynamic type error *)
   | c_wrong : Comp v
 
   (* multiple results *)
-  | c_multi : list v -> Comp v.
+  | c_multi : list v -> Comp v
+
+.
 
 #[export] Hint Constructors Comp : core.
 
 Arguments c_wrong {_}.
 Arguments c_multi {_}.
+
+(* ----------------------------------------------------------- *)
+
+(* Comp is a monad *)
 
 Definition pure_Comp {A} (x : A) : Comp A := c_multi (x :: nil).
 
@@ -95,8 +100,88 @@ Definition join_Comp {A} (m : Comp (Comp A)) : Comp A :=
 Definition bind_Comp {A B} (m : Comp A) (k : A -> Comp B) : Comp B :=
   join_Comp (fmap_Comp k m).
 
-#[global] Instance Monad_Comp : Monad Comp.
+#[export] Instance Functor_Comp : Functor Comp.
+split. exact @fmap_Comp. Defined.
+
+
+#[export] Instance Monad_Comp : Monad Comp.
 split. exact @pure_Comp. exact @bind_Comp. Defined.
+
+Lemma append_Comp_nil {A} : forall (x : Comp A), append_Comp x (c_multi nil) = x.
+Proof.
+  intros.
+  destruct x; simpl; auto.
+  rewrite app_nil_r.
+  auto.
+Qed.
+
+
+
+(* ------------------------------------------------------- *)
+
+Definition Comp_In {A} (x : A) (u : Comp A) := 
+  match u with 
+  | c_wrong => False
+  | c_multi vs => List.In x vs
+  end.
+
+Definition Comp_inj {A} (C : list (Comp (list A))) : P (Comp (P A)) :=
+  mem (List.map (fmap mem) C).
+
+Inductive Comp_Approx {A}: Comp (list A) -> Comp (P A) -> Prop :=
+  | CA_wrong : Comp_Approx c_wrong c_wrong
+  | CA_multi : forall ll lX,
+              List.Forall2 (fun l X => mem l ⊆ X) ll lX ->
+              Comp_Approx (c_multi ll) (c_multi lX).
+
+
+Definition Comp_Approx_in {A} (C : Comp (list A)) (D : P (Comp (P A))) : Prop :=
+  exists d, (d ∈ D) /\ (Comp_Approx C d).
+
+Infix "⊑c" := Comp_Approx    (at level 65).
+Infix "∈c" := Comp_Approx_in (at level 65).
+
+(* This function is ok. *)
+
+Definition split {A} (C : P (Comp A)) : P (Comp (P A)) :=
+  fun D => 
+    match D with 
+    | c_wrong => c_wrong ∈ C
+    | c_multi WS => 
+        exists (vs : list A), (c_multi vs ∈ C) /\ List.Forall2 Sets.In vs WS
+    end.
+
+
+(* Generalizes In through multi values *)
+
+Definition In2 {A} (d : Comp A) (D : P (Comp (P A))) : Prop :=
+    match d with 
+     | c_wrong => c_wrong ∈ D
+     | c_multi VS =>
+         exists WS, (c_multi WS ∈ D) /\
+            List.Forall2 Sets.In VS WS
+    end.
+
+(* ------------------------------------------------------- *)
+
+(* M is *almost* a Monad *)
+
+Definition M := fun x => P (Comp x).
+
+Definition RET {A} (x : P A) : P (Comp (P A)) :=
+  fun z => match z with 
+          | c_multi (y :: nil) => y ⊆ x
+          |  _ => False
+        end.
+
+Definition BIND {A B} (S : M A) (K : A -> M B) (t : Comp B) : Prop :=
+  exists (u : Comp A), exists (k : A -> Comp B), 
+    S u /\ t = bind u k /\ forall a, Comp_In a u -> K a (k a).
+
+(*
+#[export] Instance Monad_M : Monad M.
+split. exact @RET. exact @BIND. Defined.
+*)
 
 (* ----------------------------------------------------------- *)
 
@@ -105,7 +190,7 @@ Inductive Value : Type :=
   | v_nat : nat -> Value
 
   (* one entry in a function's table *)
-  | v_map : list Value -> Comp Value -> Value
+  | v_map : list Value -> Comp (list Value) -> Value
 
   (* trivial function value, evaluated to a value but never applied *)
   | v_fun : Value
@@ -146,8 +231,6 @@ Definition valid_Comp (C : P (Comp Value)) : Type :=
 
 (* ------------ Semantic Operators ------------------ *)
 
-Definition WRONG : P (Comp Value) := ⌈ c_wrong ⌉.
-
 Definition NAT : nat -> P Value :=
   fun j v => match v with 
           | v_nat k => j = k
@@ -171,19 +254,36 @@ Definition CONS : P Value -> P Value -> P Value :=
     end.
 
 
+(*
 Definition CONS2 : Value -> Value -> P (Comp Value) := 
   fun v w => match w with 
             | v_list u => ⌈ ret (v_list (v :: u)) ⌉
             |  _ => ⌈ c_wrong ⌉
           end.
+*)
 
 
+(* This is the key definition: what if the result of the computation 
+   diverges??? *)
+
+(*
 Definition Λ : (P Value -> P (Comp Value)) -> P Value :=
   fun f => fun v => match v with 
           | (V ↦ w) => (w ∈ f (mem V)) /\ valid_mem V  (* CBV *)
           | v_fun => True
           | _ => False
           end.
+*)
+
+
+
+Definition Λ2 : (P Value -> P (Comp (P Value))) -> P Value :=
+  fun f => fun v => match v with 
+          | (V ↦ w) => (fmap mem w ∈ (f (mem V))) /\ valid_mem V  (* CBV *)
+          | v_fun => True
+          | _ => False
+          end.
+
 
 (* ------------ APPLY ----------------- *)
 
@@ -216,15 +316,22 @@ Inductive applicable : Value -> Prop :=
 
 #[export] Hint Constructors applicable : core.
 
-Inductive APPLY : P Value -> P Value -> (Comp Value -> Prop) :=
+Inductive APPLY : P Value -> P Value -> (Comp (P Value) -> Prop) :=
   | BETA : forall D1 D2 w V,
       (V ↦ w) ∈ D1 ->
      (mem V ⊆ D2) -> valid_mem V ->
-     APPLY D1 D2 w
+     APPLY D1 D2 (fmap mem w)
+
+(* NOTE: need to incorporate eta-expansion here to order for exists
+
+  <v1 ... vn > i == (i=0;v1) | .. | (i=n;vn)
+
+*)
+ 
   | PROJ   : forall D1 D2 w VS k, 
      (v_list VS) ∈ D1 ->
      (v_nat k ∈ D2) -> nth_error VS k = Some w ->
-     APPLY D1 D2 (ret w)
+     APPLY D1 D2 (ret ⌈ w ⌉)
   | APPWRONG : forall D1 D2 x, 
       x ∈ D1 ->
       not (applicable x) ->      
@@ -243,7 +350,7 @@ Infix "▩" := APPLY (at level 90).
 Definition ADD : P Value :=
   fun w => 
     match w with 
-    | (V ↦ c_multi (v_nat k :: nil)) => 
+    | (V ↦ c_multi ((v_nat k :: nil) :: nil)) => 
         exists i j, ((v_list (v_nat i :: v_nat j :: nil)) ∈ mem V) /\ k = i + j
     | V ↦ c_wrong => 
         not (exists i j, v_list (v_nat i :: v_nat j :: nil) ∈ mem V) /\ valid_mem V
@@ -254,6 +361,8 @@ Definition ADD : P Value :=
 
 Definition Rho := Env (P Value).
 
+Definition Bottom : P Value := fun x => False.
+
 Ltac gather_atoms ::=
   let A := gather_atoms_with (fun x : vars => x) in
   let B := gather_atoms_with (fun x : var => {{ x }}) in
@@ -263,7 +372,7 @@ Ltac gather_atoms ::=
   constr:(A \u B \u C \u D \u E).
 
 Module EnvNotations.
-Notation "ρ ⋅ x" := (Env.access (fun x => False) ρ x) (at level 50).
+Notation "ρ ⋅ x" := (Env.access Bottom ρ x) (at level 50).
 Infix "⊔e" := (Env.map2 Union) (at level 60).
 Infix "⊆e" := (Env.Forall2 Included) (at level 50).
 End EnvNotations.
@@ -274,6 +383,7 @@ Import EnvNotations.
 
 Definition monotone {A}{B} (F : P A -> P B) : Set := 
   forall D1 D2, (D1 ⊆ D2) -> F D1 ⊆ F D2.
+
 (* aka sub_preserving *)
 Definition sub_reflecting {A}{B} (F : P A -> P B) : Set := 
   forall D1 D2, F D1 ⊆ F D2 -> (D1 ⊆ D2).
@@ -284,6 +394,8 @@ Definition monotone_env {A} (D : Rho -> P A) :=
 Definition finite {B} (X : P B) : Prop := 
   exists E, (X ≃ mem E) /\ E <> nil.
 
+Definition finite_env : Rho -> Prop := Env.Forall finite.
+  
 (* ------------------------------------------------------- *)
 
 Definition nonempty_env : Rho -> Type := Env.ForallT nonemptyT.
@@ -294,70 +406,157 @@ Definition sub_env : Rho -> Rho -> Prop := Env.Forall2 Included.
 
 Definition same_env : Rho -> Rho -> Prop := Env.Forall2 Same_set.
 
+
+(* ---------------------------------------------------- *)
+
+(* 
+
+ Comparison between
+
+    C : P (Comp Value)  
+
+ and
+
+    D : P (Comp (P Value))
+
+*)
+
+(* This function is lossy. Produces an empty set if 
+   *any* of the mult values are empty. 
+   We probably don't want to use it.
+*)
+Definition merge {A} (D : P (Comp (P A))) : P (Comp A) :=
+  fun C => (match C with 
+    | c_wrong => c_wrong
+    | c_multi vs => c_multi (fmap ret vs)
+    end) ∈ D.
+
+
+(* Generalizes In through multi values *)
+Definition DeepIn {A} (d : Comp (P A)) (D :  P (Comp (P A))) : Prop :=
+    match d with 
+     | c_wrong => c_wrong ∈ D
+     | c_multi VS => 
+            exists WS, (c_multi WS ∈ D) /\ List.Forall2 Ensembles.Included VS WS
+        end.
+
+(* Generalizes Included through multi values *)
+Definition DeepIncluded {A} (D1 D2 :  P (Comp (P A))) : Prop :=
+  forall (d : Comp (P A)), d ∈ D1 -> DeepIn d D2.
+
+Definition DeepSame_set {A} (D1 D2 :  P (Comp (P A))) : Prop :=
+  DeepIncluded D1 D2 /\ DeepIncluded D2 D1.
+
+Infix "∈M" := DeepIn       (at level 65).
+Infix "⊆M" := DeepIncluded (at level 65).
+Infix "≃M" := DeepSame_set (at level 65).
+
+
+
+Example DeepIn_Example : 
+  (c_multi (Bottom :: nil) ∈M  ⌈ c_multi (⌈ v_nat 0 ⌉ :: nil)⌉).
+cbv.
+ exists (⌈ v_nat 0 ⌉ :: nil).
+ split. econstructor; eauto.
+ econstructor; eauto. intros x h. inversion h.
+Qed.
+
+
+Lemma not_Bottom_Singleton :  forall v, not (Bottom ≃ ⌈ v ⌉).
+Proof.
+  intros v [h1 h2].
+  specialize (h2 v ltac:(auto)).
+  done.
+Qed.
+
+Example merge_multi : merge ⌈ c_multi (Bottom :: nil) ⌉ ≃ fun x => False.
+Proof.
+  split.
+  intros x h.
+  destruct x.
+  - inversion h.
+  - inversion h.
+    destruct l. done. simpl in H0. inversion H0. 
+    destruct l; try done. clear H2. clear H0.
+    move: (not_Bottom_Singleton v) => h1.
+    assert False. apply h1. rewrite H1. reflexivity. done.
+  - intros x h. inversion h.
+Qed.
+
+Lemma In_Singleton_Included {A} : forall (x:A) a, In x a ->  ⌈ x ⌉ ⊆ a.
+Proof.
+  intros.
+  intros y yIn. inversion yIn. subst. auto.
+Qed.
+
+#[export] Hint Resolve In_Singleton_Included : core.
+
+Example split_merge_inv_counterexample : 
+  not (c_multi (Bottom :: nil) ∈ split( merge ⌈ c_multi (Bottom :: nil) ⌉ )).
+Proof.
+  intro h.
+  move: h => [vs [h1 h2]].
+  inversion h2. done.
+Qed.
+
+Lemma merge_split : forall A (C : P (Comp A)), merge (split C) ≃ C.
+Proof.
+  intro C. split.
+  - intros c cIn.
+    destruct c; cbn in cIn; auto.
+    move: cIn => [vs [h1 h2]].
+    have EQ: (vs = l).
+    { clear C0 h1. move:vs h2. induction l; intros vs h2; inversion h2.
+      done.
+      subst. inversion H2. subst. f_equal. apply IHl. auto.
+    } 
+    subst. done.
+  - intros c cIn.
+    destruct c; cbn. auto.
+    exists l. split; auto. clear cIn. induction l. simpl. eauto.
+    econstructor; eauto. eapply in_singleton.
+Qed.
+
+(* ------------------------------------------------------------------------------- *)
+
+Definition RET2 {A} : P A -> P (Comp A) := fmap ret.
+
+(* This K wants a finite set of values from S at once 
+   so that the APPLY function can check that the domain is 
+   included in the argument. *)
+
+(* The nonempty requirement means that BIND2 is strict *)
+
+(* But this definition of bind doesn't do the cross product for the lists. *)
+Definition BIND2 {A B} (S : P (Comp A)) (K : P A -> P (Comp B)) (t : Comp B) : Prop :=
+  exists (V : P A), nonempty V /\ (RET2 V ⊆ S) /\ K V t.
+
+Definition AP {A B} (f : A -> B) ( X : P A ) : P B := 
+  fun y => exists x, (f x = y) /\ (x ∈ X).
+
+(*
+Definition BIND3 {A B} (S : P (Comp A)) (K : P A -> P (Comp B)) (t : Comp B) : Prop :=
+  
+
+
+  exists (V : P A), nonempty V /\
+     exists (k : A -> Comp B), t = bind 
+                   AP k = K
+                        AP k 
+      (* All values in V are found in S *)
+                 (forall v, v ∈ V -> Comp_In 
+
+(RET2 V ⊆ S) /\ K V t.
+*)
+
 (* ------------------------------------------------------- *)
 
 Import LCNotations.
 Open Scope tm.
 
-(* Some properties about P and M *)
-
-#[export] Instance Monad_P : Monad P :=
-  { ret  := (fun A (x : A) => ⌈ x ⌉);
-     bind := fun A B (ca : P A) (k : A -> P B) =>
-             fun b => exists a, (a ∈ ca) /\ (b ∈ k a)
-   }.
-
-#[export] Instance Functor_P : Functor P :=
-  { fmap := fun A B (f : A -> B) (x : A -> Prop) => 
-               bind x (fun y => ret (f y)) 
-  }.
-
-#[export] Instance Applicative_P : Applicative P :=
-  { pure := @ret P _;
-     ap   := fun A B (m1 :  P (A -> B)) (m2 : P A) => 
-               bind m1 (fun x1 => 
-                            bind m2 (fun x2 => 
-                                         ret (x1 x2))) 
-  }.
-
-#[export] Instance Alternative_P : Alternative P :=
-  { empty := fun A (x:A) => False ;
-    choose := fun A (p1 p2 : P A) (y : A) => 
-                 p1 y \/ p2 y
-   }.
-
-Definition M := fun x => P (Comp x).
-
-Definition Comp_In {A} (x : A) (u : Comp A) := 
-  match u with 
-  | c_wrong => False
-  | c_multi vs => List.In x vs
-  end.
-
-Definition RET {A} : A -> M A :=
-  fun x => ⌈ ret x ⌉.
-
-Definition BIND {A B} (S : M A) (K : A -> M B) (t : Comp B) : Prop :=
-  exists (u : Comp A), exists (k : A -> Comp B), 
-    S u /\ t = bind u k /\ forall a, Comp_In a u -> K a (k a).
-
-#[export] Instance Monad_M : Monad M.
-split. exact @RET. exact @BIND. Defined.
-
-
-
-
-Definition RET2 {A} : P A -> M A := fmap pure_Comp.
-
-(* This K wants a finite set of values from S at once 
-   so that the APPLY function can check that the domain is 
-   included in the argument. *)
-Definition BIND2 {A B} (S : P (Comp A)) (K : P A -> P (Comp B)) (t : Comp B) : Prop :=
-  exists V, finite V /\ (RET2 V ⊆ S) /\ K V t.
-
 (* Denotation function *)
 (* `n` is is a termination metric. *)
-Fixpoint denot_comp_n (n : nat) (a : tm) (ρ : Rho) : M Value :=
+Fixpoint denot_comp_n (n : nat) (a : tm) (ρ : Rho) : M (P Value) :=
   let fix denot_val_n (n : nat) (a : tm) (ρ : Rho) : P Value :=
   match n with
   | O => fun x => False
@@ -369,7 +568,7 @@ Fixpoint denot_comp_n (n : nat) (a : tm) (ρ : Rho) : M Value :=
 
      | abs t => 
         let x := fresh_for (dom ρ \u fv_tm t) in 
-        (Λ (fun D => (denot_comp_n m (t ^ x) (x ~ D ++ ρ))))
+        (Λ2 (fun D => (denot_comp_n m (t ^ x) (x ~ D ++ ρ))))
 
      | tcons t u => CONS (denot_val_n m t ρ) (denot_val_n m u ρ)
 
@@ -387,16 +586,16 @@ Fixpoint denot_comp_n (n : nat) (a : tm) (ρ : Rho) : M Value :=
   | S m => 
       match a with 
        | app t u   => 
-           BIND2 (denot_comp_n m t ρ) (fun v1 =>
-           BIND2 (denot_comp_n m u ρ) (fun v2 =>
-           v1 ▩ v2))
+           BIND (denot_comp_n m t ρ) (fun v1 =>
+           BIND (denot_comp_n m u ρ) (fun v2 =>
+           (v1 ▩ v2)))
 
        | tcons t u => 
-           BIND2 (denot_comp_n m t ρ) (fun v1 =>
-           BIND2 (denot_comp_n m u ρ) (fun v2 => 
-           RET2 (CONS v1 v2 )))
+           BIND (denot_comp_n m t ρ) (fun v1 =>
+           BIND (denot_comp_n m u ρ) (fun v2 => 
+           RET (CONS v1 v2 )))
 
-       | _ => RET2 (denot_val_n n a ρ)
+       | _ => RET (denot_val_n n a ρ)
      end
 
   end.
@@ -412,7 +611,7 @@ Fixpoint denot_val_n (n : nat) (a : tm) (ρ : Rho) : P Value :=
 
      | abs t => 
         let x := fresh_for (dom ρ \u fv_tm t) in 
-        (Λ (fun D => (denot_comp_n m (t ^ x) (x ~ D ++ ρ))))
+        (Λ2 (fun D => (denot_comp_n m (t ^ x) (x ~ D ++ ρ))))
 
      | tcons t u => CONS (denot_val_n m t ρ) (denot_val_n m u ρ)
 
@@ -433,11 +632,144 @@ Definition denot_val (a : tm) := denot_val_n (size_tm a) a.
 #[export] Hint Opaque denot_val : core.
 
 
+(*
+Lemma ret_In_RET {A} : forall (U V : P A),
+  U ⊆ V <-> (ret U) ∈ (RET V).
+Proof.
+  intros. 
+  unfold  RET, ret, Monad_Comp, pure_Comp.
+  cbv.
+  split.
+  + intros Ux. auto.
+  + auto.
+Qed. *)
+
+Lemma RET_monotone {A} : forall (U V : P A), 
+ U ⊆ V -> RET U ⊆ RET V. 
+Proof. 
+    intros U V h x xIn.
+    unfold Included in h.
+    destruct x; simpl in *; eauto.
+    destruct l; try done.
+    destruct l; try done.
+    unfold RET in *. cbn in *.
+    unfold Included in xIn.
+    intros x. 
+    eauto.
+Qed.
+
+Lemma RET_sub_reflecting {A} : forall (U V : P A), 
+  RET U ⊆ RET V -> U ⊆ V.
+Proof. 
+  intros U V h x xIn.
+  unfold RET in h.
+  specialize (h (c_multi (U :: nil))). cbn in h.
+  unfold Included in h.
+  eauto.
+Qed.
+
+#[export] Instance Proper_Included_RET {A} : Proper (Included ==> Included) 
+                                               (@RET (P A)).
+unfold Proper. intros x1 y1 E1. eapply RET_monotone. auto. Qed.
+
+#[export] Instance Proper_Same_RET {A} : Proper (Same_set ==> Same_set) (@RET (P A)).
+unfold Proper. intros x1 y1 E1. split. eapply RET_monotone. rewrite E1. reflexivity.
+eapply  RET_monotone. rewrite E1. reflexivity.
+Qed.
+
+Lemma bind_ret_Comp : forall {A B} (x : A) (k : A -> Comp B), 
+    bind (ret x) k = k x.
+Proof.
+  intros.
+  cbv.
+  destruct (k x); auto.
+  f_equal.
+  eapply app_nil_r.
+Qed. 
+
+Lemma BIND_RET : forall {A B} (x : P A) (k : P A -> M B), 
+    monotone k -> 
+    BIND (RET x) k ≃ k x.
+Proof. intros. unfold BIND, RET.
+repeat split.
++ intros y.
+  move =>[U [h1 [h2 [h3 h4]]]]. unfold M in k.
+  subst.
+  destruct U; try done.
+  destruct l; try done.
+  destruct l; try done.
+  cbn.
+  specialize (h4 p ltac:(cbv;eauto)).
+  rewrite append_Comp_nil.
+  eapply H; eauto.
++ intros y yIn.
+  exists (c_multi (x :: nil)).
+  exists (fun _ => y).
+  repeat split.
+  reflexivity.
+  rewrite bind_ret_Comp.
+  reflexivity.
+  intros a aIn.
+  inversion aIn. subst. auto. inversion H0.
+Qed.
+
+(*
+Lemma DeepIn_In {A} : forall (x : Comp (P A)) D, x ∈ D -> x ∈M D.
+Proof. 
+  intros.
+  destruct x; simpl.
+  done.
+  exists l. split; auto. reflexivity.
+  left. auto.
+Qed.
+*)
+Lemma BIND_mono {A B} : forall (D1 D2 : P (Comp A)) (K1 K2 : A -> P (Comp B)),
+  D1 ⊆ D2 -> (forall x, K1 x ⊆ K2 x) ->
+  BIND D1 K1 ⊆ BIND D2 K2.
+Proof. 
+  intros.
+  unfold BIND.
+  move=> x [U [h1 [h2 [-> h4]]]].
+  destruct U; simpl.
+  -  exists c_wrong.
+     exists h1.
+     split.
+     specialize (H _ h2).
+     simpl in H. done.
+     split.
+     cbv.
+     done.
+     intros a aIn.
+     specialize (h4 _ aIn).
+     specialize (H0 a). unfold DeepIncluded in H0.
+     specialize (H0 (h1 a) h4).
+     eauto.
+  - exists (c_multi l).
+    exists h1. 
+    repeat split; eauto.
+    eapply H; auto.
+    intros a aIn. eapply H0. eapply h4. auto.
+Qed.
+
+#[export] Instance Proper_Included_BIND {A B} : Proper (Included ==> Logic.eq ==> Included) (@BIND A B).
+intros x1 y1 E1 x2 y2 ->. 
+eapply BIND_mono; eauto. reflexivity.
+Qed. 
+
+#[export] Instance Proper_Same_BIND {A B} : Proper (Same_set ==> Logic.eq ==> Same_set) (@BIND A B).
+unfold Proper. intros x1 y1 E1 x2 y2 ->. split. eapply BIND_mono. rewrite E1. reflexivity. reflexivity.
+eapply  BIND_mono. rewrite E1. reflexivity. reflexivity.
+Qed.
+  
+
+
+(*
+
 
 Require Import Coq.Logic.PropExtensionality.
 
 Lemma ret_In_RET2 : forall {A} (U : P A) x,
-  x ∈ U <-> ret x ∈ RET2 U.
+  x ∈ U <-> ret x ε RET2 U.
 Proof.
   intros. 
   unfold ret, RET2, fmap, Monad_Comp, Functor_P, bind, Monad_P, Ensembles.In.
@@ -480,7 +812,7 @@ Qed.
 
 Lemma BIND2_RET2 : forall {A B} (x : P A) (k : P A -> M B), 
     monotone k 
-    -> finite x
+    -> nonempty x
     -> BIND2 (RET2 x) k ≃ k x.
 Proof. intros. unfold BIND2, RET2.
 repeat split.
@@ -519,3 +851,4 @@ eapply  BIND2_mono. rewrite E1. reflexivity. reflexivity.
 Qed.
   
 
+*)
